Towards termination of complete LF language

Normalization/LF_Complete.v
@@ -57,11 +57,11 @@ apply lc_t_subst_t_LF_bound; auto.
 eapply IHM1; eauto.
 eapply IHM; eauto.
 eapply IHM; eauto.
-constructor; auto.
+(*constructor; auto.
 unfold open_LF; apply lc_t_subst_t_LF_bound; auto.
 eapply IHM1; eauto.
 constructor; auto. apply closed_t_succ_LF; auto.
-Qed.
+Qed. *) Admitted.
 
 Definition normal_form (M: te_LF) := value_LF M.
 
@@ -501,17 +501,16 @@ match A with
   forall N,
     lc_t_LF N ->
     Red N A1 ->
-    Red (appl_LF M N) A2 /\
     forall K,
       ContLC K ->
       RedCont K A2 ->
       WTCont K (appl_LF M N)
 
-| tbox A1 => WT M /\ Red (unbox_LF M) A1
-(*             forall K,
+| tbox A1 => WT M /\
+             forall K,
                ContLC K ->
                RedCont K A1 ->
-               WTCont K (unbox_LF M) *)
+               WTCont K (unbox_LF M)
 | tdia A1 =>
   forall K,
     ContLC K ->
@@ -674,7 +673,7 @@ destruct H6 as (V', (H6, H7)).
 apply WT_steps with (M:=ContAppl K (here_LF (letdia_LF A (here_LF V') N))).
 apply steps_KApplSteps; auto.
 repeat constructor; auto. apply lc_t_steps_LF with (n:=0) in H7; auto.
-skip.
+skip. (* from H7 *)
 apply H1.
 Focus 2. repeat constructor; auto. apply lc_t_steps_LF with (n:=0) in H7; auto.
 apply property_3 with (M':=[V'//bte 0] N).
@@ -684,6 +683,83 @@ constructor; auto. apply lc_t_steps_LF with (n:=0) in H7; auto.
 apply H2; auto. apply lc_t_steps_LF with (n:=0) in H7; auto.
 apply property_2_steps with (M:=V); auto.
 Qed.
+
+Lemma steps_val_here:
+forall M V,
+  steps_LF (here_LF M) V ->
+  value_LF V ->
+  exists M0, V = here_LF M0.
+intros; remember (here_LF M) as M1;
+generalize dependent M; induction H; intros; subst.
+inversion H; subst; eexists; eauto.
+inversion H; subst.
+destruct IHsteps_LF with M'0; auto; subst; eexists; eauto.
+Qed.
+
+Lemma steps_letdia:
+forall M M', steps_LF M M' ->
+forall A N, lc_t_LF M -> lc_t_n_LF 1 N ->
+            steps_LF (letdia_LF A M N) (letdia_LF A M' N).
+intros M M' H; induction H; intros; simpl in *.
+constructor; constructor; auto.
+apply multi_step_LF with (M':=letdia_LF A M' N); auto.
+constructor; auto. apply IHsteps_LF; auto. apply lc_t_step_LF in H; auto.
+Qed.
+
+Lemma steps_here:
+forall M M', steps_LF M M' -> lc_t_LF M -> steps_LF (here_LF M) (here_LF M').
+intros; induction H; simpl in *.
+repeat constructor; auto.
+apply multi_step_LF with (M':=here_LF M').
+repeat constructor; auto.
+apply IHsteps_LF; apply lc_t_step_LF in H; auto.
+Qed.
+
+Lemma Lemma_6:
+forall M,
+  lc_t_LF M -> WT M ->
+  forall N K A, lc_t_n_LF 1 N -> ContLC K ->
+  WT (ContAppl K (here_LF (N ^t^ M))) ->
+  WT (ContAppl K (here_LF (letdia_LF A (here_LF M) N))).
+intros M LC H; induction H; intros.
+apply WT_step_back with (N:=ContAppl K (here_LF (N ^t^ V))); auto.
+apply Step_KApplStep; auto.
+repeat constructor; auto.
+repeat constructor; auto.
+destruct H as (V, (H, H3)).
+apply WT_steps_back
+with (N:=(ContAppl K (here_LF (letdia_LF A (here_LF V) N)))).
+apply steps_KApplSteps; auto.
+repeat constructor; auto.
+apply steps_here; auto.
+apply steps_letdia; auto.
+apply steps_here; auto. constructor; auto.
+repeat constructor; auto.
+apply WT_step_back with (N:=ContAppl K (here_LF (N ^t^ V))).
+Focus 2.
+apply Step_KApplStep; auto.
+repeat constructor; auto; eapply lc_t_steps_LF in H3; eauto.
+repeat constructor; auto.
+apply lc_t_steps_LF with (n:=0) in H3; auto.
+apply lc_t_steps_LF with (n:=0) in H3; auto.
+Admitted.
+
+Lemma Lemma_7:
+forall K M A N B,
+  lc_t_n_LF 1 N -> lc_t_LF M ->
+  Red M (<*>A) ->
+  (forall P, Red P A -> Red (N ^t^ P) B) ->
+  RedCont K B ->
+  ContLC K ->
+  WT (ContAppl K (here_LF (letdia_LF A M N))).
+intros; simpl in *; unfold RedCont in *.
+assert (RedCont (ConsK K N A B) A); unfold RedCont; intros.
+simpl.
+apply Lemma_6; auto.
+apply property_1 in H5; auto.
+apply H3. apply H2; auto. unfold open_LF; apply lc_t_subst_t_LF_bound; auto.
+unfold RedCont in *. simpl in *.
+Admitted.
 
 Lemma SL_hyp:
 forall L G Gamma v A,
@@ -700,6 +776,25 @@ assert (Mem (v, A) (map fst_ L)).
 apply Mem_find_var_type in H3; auto. destruct H3.
 simpl; rewrite e; apply H1 with v.
 apply find_var_Mem; auto.
+Qed.
+
+Lemma WT_subst_val:
+forall M N v,
+lc_t_LF M -> lc_t_LF N ->
+value_LF N -> WT M -> WT [M // v]N.
+intros. generalize dependent M;
+generalize dependent v;
+induction H1; intros; simpl.
+constructor; constructor; auto.
+constructor; constructor; auto.
+inversion H0; subst;
+rewrite <- WT_here; auto.
+inversion H0; subst.
+destruct v. destruct n.
+apply lc_t_subst_t_LF_bound; auto;
+apply closed_t_succ_LF; auto.
+rewrite closed_subst_t_bound_LF with (n:=0); auto; omega.
+apply lc_t_subst_t_LF_free; auto.
 Qed.
 
 Theorem main_theorem:
@@ -733,8 +828,8 @@ unfold RedCont in *; apply H5; auto.
 unfold RedCont in *; apply H6; auto;
 [split | inversion LC; constructor; apply lc_SL; auto];
 [repeat constructor | intros].
-split. skip. (* !!! *)
-intros; apply WT_step_back with (N:=ContAppl K0 (here_LF ((SL L0 M) ^t^ N)));
+unfold WTCont;
+apply WT_step_back with (N:=ContAppl K0 (here_LF ((SL L0 M) ^t^ N)));
 unfold open_LF in *;
 assert (exists x, x \notin L \u used_vars_te_LF (SL L0 M) \u FV_L L0
        \u  from_list (map fst_ (map fst_ L0))  \u from_list nil)
@@ -766,60 +861,9 @@ apply notin_Mem; auto. apply notin_Mem; auto.
 rewrite SL_bte_subst; auto. rewrite SL_extend; auto.
 apply notin_Mem; auto. apply notin_Mem; auto.
 (* appl *)
-inversion LC; subst.
-remember (SL L M) as M';
-remember (SL L N) as N'.
-assert (WT (ContAppl (IdK (A--->B)) (here_LF M'))).
-  subst; apply IHHT1; auto. constructor.
-  unfold RedCont; intros; simpl. rewrite <- WT_here.
-  apply property_1 in H5; auto. auto.
-simpl in H5. apply WT_here in H5. assert (WT' M') by skip.
-destruct H6 as (V, (H6, H7)).
-apply WT_steps_back with (N:=ContAppl K (here_LF ([N'//bte 0] V))).
-apply steps_KApplSteps; auto.
-repeat constructor; subst; apply lc_SL; auto.
-skip (* from H7 *).
-
-(* These two are all I need *)
-assert (Red (SL L M) (A ---> B)). simpl; split.
-  (* WT *)
-  assert (WT (ContAppl (IdK (A--->B)) (here_LF (SL L M)))).
-    apply IHHT1; auto; simpl. constructor.
-    unfold RedCont; intros; simpl. rewrite <- WT_here.
-    apply property_1 in H5; auto. auto.
-  simpl in H5. apply WT_here; auto; apply lc_SL; auto.
-  (* ... *)
-  intros; unfold WTCont in *.
-
-assert (Red (SL L N) A). skip.
-simpl in H5; destruct H5; apply H7; auto;
-apply lc_SL; inversion LC; auto.
-
-simpl.
-inversion LC; subst.
-apply WT_ContAppl_appl with B.
-assert (WT (ContAppl (IdK B) (here_LF (SL L M)))).
-apply IHHT1; auto; intros. constructor.
-destruct H5.
-simpl. rewrite <- WT_here. rewrite <- WT_here. auto.
-auto. constructor; auto.
-simpl in H5.
-apply WT_here. apply lc_SL; auto. apply WT_here.
-constructor; apply lc_SL; auto.
-auto.
-assert (WT (ContAppl (IdK A) (here_LF (SL L N)))).
-apply IHHT2; auto; intros. constructor.
-simpl. apply property_1 in H5.
-rewrite <- WT_here. rewrite <- WT_here. auto.
-auto. constructor; auto.
-auto.
-simpl in H5.
-apply WT_here. apply lc_SL; auto. apply WT_here.
-constructor; apply lc_SL; auto.
-auto.
-unfold RedCont; auto.
+skip. (* !!! *)
 (* box *)
-inversion LC; subst;
+unfold RedCont in *; inversion LC; subst;
 apply H4; [ | constructor; apply lc_SL; auto];
 split; [ repeat constructor | intros].
 apply WT_step_back with (N:=ContAppl K0 (here_LF (SL L M))).
@@ -830,40 +874,14 @@ repeat constructor; apply lc_SL; auto.
 constructor. repeat constructor; apply lc_SL; auto.
 constructor; apply lc_SL; auto.
 (* unbox *)
-inversion LC; subst.
-apply WT_ContAppl_unbox with A.
-assert (WT (ContAppl (IdK A) (here_LF (SL L M)))).
-apply IHHT; auto; intros. constructor.
-destruct H5.
-simpl. rewrite <- WT_here. rewrite <- WT_here. auto.
-auto. constructor; auto.
-simpl in H5.
-apply WT_here. apply lc_SL; auto. apply WT_here.
-constructor; apply lc_SL; auto.
-auto.
-unfold RedCont; auto.
+skip. (* !!! *)
 (* unbox-fetch *)
-inversion LC; subst.
-apply WT_ContAppl_unbox with A.
-assert (WT (ContAppl (IdK A) (here_LF (SL L M)))).
-apply IHHT; auto; intros.
-rew_map in *; simpl; rewrite <-  H1; rew_concat; auto. permut_simpl.
-replace (Gamma ++ concat G) with (concat (Gamma::G)) by (rew_concat; auto).
-apply PPermut_concat_permut; rewrite <- H; PPermut_LF_simpl.
-constructor.
-destruct H6.
-simpl. rewrite <- WT_here. rewrite <- WT_here. auto.
-auto. constructor; auto.
-simpl in H6.
-apply WT_here. apply lc_SL; auto. apply WT_here.
-constructor; apply lc_SL; auto.
-auto.
-unfold RedCont; auto.
+skip. (* !!! *)
 (* here *)
-apply H4; [ intros | inversion LC; constructor; apply lc_SL; auto].
+apply H4; [ simpl; intros | inversion LC; constructor; apply lc_SL; auto];
 apply IHHT; inversion LC; auto.
 (* get-here *)
-apply H5; [ intros | inversion LC; constructor; apply lc_SL; auto].
+apply H5; [ simpl; intros | inversion LC; constructor; apply lc_SL; auto].
 apply IHHT; inversion LC; subst; auto.
 rew_map in *; simpl; rewrite <-  H1; rew_concat; auto. permut_simpl.
 replace (Gamma ++ concat G) with (concat (Gamma::G)) by (rew_concat; auto).
@@ -872,878 +890,52 @@ apply PPermut_concat_permut; rewrite <- H; PPermut_LF_simpl.
 inversion LC; subst.
 replace (ContAppl K (here_LF (letdia_LF A (SL L0 M) (SL L0 N)))) with
  (ContAppl (ConsK K (SL L0 N) A B) (SL L0 M)) by (simpl; auto).
-apply WT_here.
-apply lc_ContAppl.
-constructor; auto; apply lc_SL; auto. apply lc_SL; auto.
-
-remember (ConsK K (SL L0 N) A B) as K'.
-assert (WT (ContAppl K' (here_LF (SL L0 M)))).
-apply IHHT; auto.
-subst; constructor; auto; apply lc_SL; auto.
-intros.
-
-subst; simpl.
-
-apply property_1 with B.
-skip.
-replace
-
-
-
-
-Focus 9.
-inversion LC; subst.
-replace (ContAppl K (here_LF (letdia_LF A (SL L0 M) (SL L0 N)))) with
- (ContAppl (ConsK K (SL L0 N) A B) (SL L0 M)) by (simpl; auto).
-assert (exists v, v \notin L \u  used_vars_te_LF (SL L0 N) \u
-       from_list (map fst_ (map fst_ L0)))
-  by apply Fresh. destruct H6.
-assert (Red (ContAppl K (here_LF (SL L0 (N ^t^ hyp_LF (fte x))))) B0).
-  apply H with (G':= ((x, A) :: nil) :: G); auto.
-  skip. skip.
-assert (Red (ContAppl (IdK B) (here_LF (SL L0 (N ^t^ hyp_LF (fte x))))) B).
-  apply H with (G':= ((x, A) :: nil) :: G); auto.
-  skip. skip.  constructor. unfold RedCont; intros; simpl.
-  rewrite <- WT_here. apply property_1 in H8; auto. auto.
-unfold open_LF in *. simpl in H8.
-assert (Red (ContAppl (ConsK K (SL L0 N) A B) (here_LF (SL L0 M))) B0).
-  apply IHHT; auto.
-  constructor; auto; apply lc_SL; auto.
-  apply RedCont_cons; auto.
-  apply lc_SL; auto.
-  intros.
-  rewrite subst_t_neutral_free_LF with (v:=x).
-  rewrite SL_bte_subst; [ | apply notin_Mem |]; eauto.
-  Focus 2. auto.
-  rewrite <- SL_extend with (A:=A).
-  assert (Red (ContAppl (IdK B) (here_LF (SL ((x, A, P) :: L0)
-                                             (N ^t^ hyp_LF (fte x))))) B).
-  apply H with (G':= ((x, A) :: nil) :: G); auto.
-  skip. constructor; [rewrite Mem_nil_eq | apply OkL_fresh]; auto. skip.
-  skip.
-  intros; rewrite Mem_cons_eq in *; destruct H13; eauto; inversion H13;
-  subst; auto.
-  intros; rewrite Mem_cons_eq in *; destruct H13; eauto; inversion H13;
-  subst; auto. skip.
-  constructor.
-  unfold RedCont; intros; simpl.
-  rewrite <- WT_here. apply property_1 in H13; auto. auto.
-  simpl in H13; unfold open_LF in *.
-  skip. (* close enough *) skip. skip.
-skip.
-
-
-
-
-apply WT_ContAppl_letdia with B.
-assert (WT (ContAppl (IdK A) (here_LF (SL L0 M)))).
-apply IHHT; auto; intros. constructor.
-simpl. rewrite <- WT_here. rewrite <- WT_here. auto.
-auto. constructor; auto.
-simpl in H5.
-apply WT_here. apply lc_SL; auto. apply WT_here.
-constructor; apply lc_SL; auto.
-auto.
-unfold RedCont; auto.
-
-
-
-
-
-
-
-
-
-
-
-
-
-
-
-
-
-
-
-
-
-
-
-
-
-
-
-
-
-
-
-
-
-
-
-
-
-
-
-
-
-
-
-
-
-
-
-
-
-
-
-
-
-
-
-
-
-
-
-
-
-
-
-
-
-
-
-
-
-
-
-
-
-
-
-
-
-
-
-
-
-
-
-
-
-
-
-
-
-
-
-
-
-Focus 9.
-apply step_WT; intros.
-
-simpl in *.
-(* here (letdia x = m in n ) -> letdia x = m in here n*)
-(* letdia y = (letdia x = m in n ) in p - > letdia x =m in letdia y= here n in p *)
-
-(*
-Lemma lc_t_subst_t_LF_bound:
-forall M N n,
-  lc_t_n_LF n N ->
-  lc_t_n_LF (S n) M ->
-  lc_t_n_LF n ([N//bte n] M).
-induction M; intros; simpl in *; inversion H0; subst; repeat case_if;
-try constructor; eauto.
-assert (n <> v0) by (intro; subst; elim H1; auto); omega.
-eapply IHM; auto; apply closed_t_succ_LF; auto.
-eapply IHM2; auto; apply closed_t_succ_LF; auto.
-Qed.
-
-Lemma lc_t_step_LF:
-forall M N,
-  lc_t_LF M ->
-  M |-> N ->
-  lc_t_LF N.
-induction M; intros; inversion H0; inversion H; subst; try constructor; eauto.
-apply lc_t_subst_t_LF_bound; auto.
-eapply IHM1; eauto.
-eapply IHM; eauto.
-eapply IHM; eauto.
-unfold open_LF; apply lc_t_subst_t_LF_bound; auto.
-eapply IHM1; eauto.
-Qed.
-
-Lemma WT_appl:
-forall M N,
-  lc_t_LF (appl_LF M N) ->
-  WT (appl_LF M N) ->
-  WT M.
-intros;
-remember (appl_LF M N) as T;
-generalize dependent M;
-generalize dependent N;
-induction H0; intros; subst;
-[ inversion H0 |
-  assert (neutral_LF M0 \/ value_LF M0) by apply neutral_or_value_LF];
-destruct H2;
-[ inversion H; subst |
-  constructor; auto];
-apply step_WT; intros;
-apply H1 with (N0:=appl_LF N0 N) (N:=N).
-constructor; eauto.
-apply lc_t_step_LF with (M:=appl_LF M0 N); auto; constructor; auto.
-auto.
-Qed.
-
-Lemma WT_box:
-forall M,
-  lc_t_LF (unbox_LF M) ->
-  WT (unbox_LF M) ->
-  WT M.
-intros; remember (unbox_LF M) as T;
-generalize dependent M;
-induction H0; intros; subst;
-[ inversion H0 |
-  assert (neutral_LF M0 \/ value_LF M0) by apply neutral_or_value_LF];
-destruct H2; [ inversion H; subst | constructor; auto];
-apply step_WT; intros;
-apply H1 with (N := unbox_LF N).
-constructor; inversion H; auto.
-apply lc_t_step_LF with (M:=unbox_LF M0); auto; constructor; auto.
-auto.
-Qed.
-
-Lemma WT_here:
-forall M,
-  lc_t_LF (here_LF M) ->
-  WT (here_LF M) ->
-  WT M.
-intros;
-remember (here_LF M) as T;
-generalize dependent M;
-induction H0; intros; subst.
-inversion H0; subst; constructor; auto.
-assert (neutral_LF M0 \/ value_LF M0) by apply neutral_or_value_LF.
-destruct H2;
-[ inversion H; subst |
-  constructor; auto].
-apply step_WT; intros;
-apply H1 with (N:=here_LF N).
-constructor; eauto.
-apply lc_t_step_LF with (M:=here_LF M0); auto; constructor; auto.
-auto.
-Qed.
-
-Theorem WT_step:
-forall M M',
-  WT M ->
-  M |-> M' ->
-  WT M'.
-intros; inversion H; subst.
-apply value_no_step_LF with (N:=M') in H1; contradiction.
-apply H1; auto.
-Qed.
-
-Lemma Step_KApplStep:
-forall K M M',
-  ContLC K ->
-  lc_t_LF M ->
-  M |-> M' ->
-  ContAppl K M |-> ContAppl K M'.
-induction K; intros; simpl in *.
-constructor; auto.
-inversion H; subst.
-assert ((letdia_LF M (here_LF t)) |-> (letdia_LF M' (here_LF t))).
-   constructor; auto; constructor; auto.
-apply IHK in H2; auto.
-constructor; auto; constructor; auto.
-Qed.
-
-(* CR 2 *)
-Theorem property_2:
-forall A M M'
-  (HRed: Red M A)
-  (H_lc_t: lc_t_LF M)
-  (HStep: M |-> M'),
-  Red M' A.
-induction A; intros; simpl in *; intros.
-(* base type *)
-inversion HRed; subst;
-[apply value_no_step_LF with (N:=M') in H; contradiction | apply H; auto].
-(* arrow type *)
-apply IHA2 with (M:=appl_LF M N); auto.
-constructor; auto.
-constructor; auto.
-(* box type *)
-apply IHA with (M:=unbox_LF M); auto; constructor; eauto.
-(* dia type *)
-specialize HRed with K B.
-assert (ContLC K) by auto;
-apply HRed in H; auto.
-apply WT_step with (M:=ContAppl K M); auto.
-apply Step_KApplStep; auto.
-Qed.
-
-Lemma WT_N_WT_here:
-forall N,
-  WT N -> WT (here_LF N).
-intros; induction H; subst.
-constructor; constructor; auto.
-apply step_WT; intros.
-inversion H1; subst.
-apply H0 in H4; auto.
-Qed.
-
-Lemma lc_ContAppl:
-forall K M,
-  ContLC K-> lc_t_LF M -> lc_t_LF (ContAppl K M).
-induction K; intros; simpl in *.
-constructor; auto.
-inversion H; subst.
-apply IHK with (M:=(letdia_LF M (here_LF t))) in H3; auto;
-constructor; auto; constructor; auto.
-Qed.
-
-Lemma neutral_ContAppl:
-forall K M,
-  neutral_LF M ->
-  neutral_LF (ContAppl K M).
-induction K; intros; simpl in *.
-constructor; auto.
-apply IHK; constructor; constructor.
-Qed.
-
-Lemma neutral_not_value:
-forall M,
-  neutral_LF M -> ~ value_LF M.
-induction M; intros; intro; try inversion H0; subst; inversion H; subst.
-apply IHM in H3; contradiction.
-Qed.
-
-Lemma step_neutral_ContAppl:
-forall K M N,
-  neutral_LF M ->
-  ContAppl K M |-> N ->
-  (exists M', N = ContAppl K M' /\ M |-> M').
-induction K; intros; simpl in *.
-inversion H0; subst; eexists; split; eauto.
-destruct IHK with (M:=(letdia_LF M (here_LF t))) (N:=N).
-constructor; constructor.
-auto.
-destruct H1.
-inversion H2; subst.
-inversion H; subst; apply neutral_not_value in H3; contradiction.
-eexists; split; eauto.
-Qed.
-
-(* CR1 + CR3 *)
-Theorem reducibility_props:
-forall A M
-  (H_lc_t: lc_t_LF M),
-  (Red M A -> WT M)
-  /\
-  (neutral_LF M -> (forall M', M |-> M' -> Red M' A) -> Red M A).
-assert (exists (x:var), x \notin \{}) as nn by apply Fresh; destruct nn; auto;
-induction A; intros; split; simpl in *.
-(* base type *)
-auto.
-intros; apply step_WT; auto.
-(* arrow type *)
-intros.
-(* Create variable of type A1 *)
-assert (forall x, nil |= (x, A1) :: nil |- hyp_LF (fte x) ::: A1).
-intros; constructor.
-unfold ok_Bg_LF; rew_concat; constructor;
-[rewrite Mem_nil_eq | constructor]; auto.
-apply Mem_here.
-assert (forall x, neutral_LF (hyp_LF x)) by (intros; constructor).
-assert (forall x, WT (hyp_LF x))
-  by (intros; apply step_WT; intros; inversion H3).
-assert (forall x, Red (hyp_LF (fte x)) A1).
-  intros; apply IHA1; auto.
-  constructor.
-  intros; inversion H4.
-assert (forall x, Red (appl_LF M (hyp_LF (fte x))) A2).
-intros; eapply H0; auto; constructor.
-assert (forall x, WT (appl_LF M (hyp_LF (fte x)))).
-intros; eapply IHA2; eauto; constructor; auto; constructor.
-(* From strong_norm (appl_L M (hyp_L x)) w deduce strong_norm M w *)
-eapply WT_appl; auto; constructor; auto; constructor.
-intros; apply IHA2; try constructor; auto; intros; simpl in *.
-inversion H2; subst; inversion H0; eapply H1; eauto.
-(* box type *)
-intros; apply WT_box.
-constructor; auto.
-apply IHA; [constructor | ]; auto.
-intros; apply IHA; try constructor; auto; intros;
-inversion H2; subst; [inversion H0 | ]; apply H1; auto.
-(* dia type *)
-intros.
-assert (WT (ContAppl (IdK A) M)).
-apply H0 with (B:=A).
-constructor.
-constructor.
-intros. simpl.
-apply IHA in H2.
-apply WT_N_WT_here; apply WT_N_WT_here; destruct H2; auto.
-simpl in H1.
-apply WT_here.
-constructor; auto.
-auto.
-intros.
-apply step_WT; intros; apply step_neutral_ContAppl in H5; auto;
-destruct H5; destruct H5;
-subst; apply H1 with B; auto.
-Grab Existential Variables.
-auto.
-Qed.
-
-Lemma property_1:
-forall A M
-  (H_lc: lc_t_LF M),
-  Red M A -> WT M.
-intros; eapply reducibility_props; eauto.
-Qed.
-
-Lemma property_3:
-forall A M
-  (H_lc: lc_t_LF M),
-  neutral_LF M ->
-  (forall M', M |-> M' ->
-    Red M' A) ->
-   Red M A.
-intros; eapply reducibility_props; eauto.
-Qed.
-
-Lemma reducible_abstraction:
-forall A N B
-  (lc_N: lc_t_LF (lam_LF A N))
-  (HT: forall M,
-    lc_t_LF M ->
-    Red M A ->
-    Red ([M// bte 0] N) B),
-  Red (lam_LF A N) (A ---> B).
-simpl; intros;
-apply property_3;
-repeat constructor; auto.
-inversion lc_N; auto.
-intros; inversion H; subst.
-apply HT; auto.
-inversion H5.
-Qed.
-
-Lemma reducible_box:
-forall A M
-  (lc_M: lc_t_LF M)
-  (HT: Red M A),
-  Red (box_LF M) ([*]A).
-simpl; intros;
-apply property_3;
-repeat constructor; auto.
-intros; inversion H; subst; auto.
-inversion H2.
-Qed.
-
-Fixpoint find_var (L: list (var * ty * te_LF)) (x:var) :
-                     option (var * ty * te_LF) :=
-match L with
-| nil => None
-| (v, A, M) :: L' =>
-  if (eq_var_dec x v) then Some (v, A, M) else find_var L' x
-end.
-
-Fixpoint SL (L: list (var * ty * te_LF)) M :=
-match M with
-| hyp_LF (bte v) => M
-| hyp_LF (fte v) =>
-  let x := find_var L v in
-  match x with
-    | Some (v, A, M) => M
-    | None => hyp_LF (fte v)
-  end
-| lam_LF A M => lam_LF A (SL L M)
-| appl_LF M N => appl_LF (SL L M) (SL L N)
-| box_LF M => box_LF (SL L M)
-| unbox_LF M => unbox_LF (SL L M)
-| here_LF M => here_LF (SL L M)
-| letdia_LF M N => letdia_LF (SL L M) (SL L N)
-end.
-
-Lemma Mem_concat_mem_elem:
-forall G (e:var*ty),
-  Mem e (concat G) ->
-  exists (l: ctx_LF), Mem l G /\ Mem e l.
-induction G; intros; rew_concat in *.
-rewrite Mem_nil_eq in H; contradiction.
-rewrite Mem_app_or_eq in H; destruct H.
-exists a; split; auto; apply Mem_here.
-destruct (IHG e); auto; destruct H0; exists x; split; auto.
-rewrite Mem_cons_eq; right; auto.
-Qed.
-
-Lemma ok_LF_Mem_Mem_eq':
-  forall (G : ctx_LF)(v : var) (A B : ty),
-    ok_LF G nil  ->
-    Mem (v, A) G -> Mem (v,B) G ->
-    A = B.
-induction G; intros.
-rewrite Mem_nil_eq in H0; contradiction.
-rewrite Mem_cons_eq in *; destruct H0; destruct H1; subst.
-inversion H1; subst; auto.
-inversion H; subst; apply Mem_split in H1; destruct H1 as (hd, (tl, H1));
-assert (hd & (v, B) ++ tl *=* (v, B) :: hd ++ tl) by permut_simpl;
-rewrite H1 in H6; apply ok_LF_permut with (G':= (v, B) :: hd ++ tl) in H6;
-auto; inversion H6; subst; elim H8; apply Mem_here.
-inversion H; subst; apply Mem_split in H0; destruct H0 as (hd, (tl, H0));
-assert (hd & (v, A) ++ tl *=* (v, A) :: hd ++ tl) by permut_simpl;
-rewrite H0 in H6; apply ok_LF_permut with (G':= (v, A) :: hd ++ tl) in H6;
-auto; inversion H6; subst; elim H8; apply Mem_here.
-eapply IHG; eauto.
-inversion H; subst; eapply ok_LF_used_weakening; eauto.
-Qed.
-
-Lemma SL_hyp:
-forall L G Gamma v A,
-  concat (Gamma::G) *=* map fst_ L ->
-  (forall a b c, Mem (a, b, c) L -> Red c b) ->
-  G |= Gamma |- hyp_LF (fte v) ::: A ->
-  Red (SL L (hyp_LF (fte v))) A.
-induction L; intros; rew_map in *.
-symmetry in H; apply permut_nil_eq in H; rew_concat in *;
-symmetry in H; apply nil_eq_app_inv in H; destruct H; subst;
-inversion H1; subst; rewrite Mem_nil_eq in *; contradiction.
-destruct a; destruct p; inversion H1; subst; simpl in *.
-case_if.
-assert (A = t0).
-unfold ok_Bg_LF in *.
-apply ok_LF_Mem_Mem_eq' with (concat (Gamma::G)) v0; auto;
-[rew_concat; rewrite Mem_app_or_eq; left; auto | ].
-apply Mem_permut with (l:=(v0,t0) :: map fst_ L); [symmetry; auto |
-apply Mem_here].
-subst; apply H0 with v0; apply Mem_here.
-assert (concat (Gamma :: G) *=* (v0, t0) :: map fst_ L) by auto;
-symmetry in H; apply permut_split_head in H;
-destruct H as (hd, (tl, H)).
-destruct Mem_concat_mem_elem with (e:=(v0, t0)) (G:=Gamma::G).
-apply Mem_permut with (l:=(v0,t0) :: map fst_ L); [symmetry; auto |];
-apply Mem_here. destruct H4.
-apply Mem_split in H4.
-apply Mem_split in H6.
-destruct H6 as (l0, (l1,H6)).
-destruct H4 as (G0, (G1, H4)); subst.
-destruct G0; rew_app in *.
-inversion H4; subst. apply IHL with G1 (l0++l1).
-rew_concat in *.
-apply permut_cons_inv with (a:=(v0,t0)).
-rewrite <- H3. permut_simpl.
-intros; apply H0 with a; rewrite Mem_cons_eq; right; auto.
-constructor.
-eapply ok_Bg_LF_permut_first_tail in Ok; eauto; permut_simpl.
-rewrite Mem_app_or_eq in *; destruct H5; auto; rewrite Mem_cons_eq in *;
-destruct H5; auto; inversion H5; subst; elim H2; auto.
-inversion H4; subst.
-apply IHL with (G0 ++ (l0 ++ l1) :: G1) c.
-rew_concat in *. apply permut_cons_inv with (a:=(v0,t0)).
-rewrite <- H3. permut_simpl.
-intros; apply H0 with a; rewrite Mem_cons_eq; right; auto.
-constructor; auto.
-assert (c :: G0 ++ (l0 ++ (v0, t0) :: l1) :: G1 ~=~
-        ((l0++(v0, t0) :: l1) :: c :: G0 ++ G1)).
-PPermut_LF_simpl; constructor; auto; permut_simpl.
-rewrite H6 in Ok.
-eapply ok_Bg_LF_permut_first_tail with (x:=v0)(A:=t0) (C':=l0++l1)in Ok; eauto.
-Focus 2. permut_simpl.
-apply ok_Bg_LF_PPermut with (G:=(l0 ++ l1) :: c :: G0 ++ G1); auto;
-PPermut_LF_simpl.
-Qed.
-
-Lemma closed_t_succ:
-forall M n,
-  lc_t_n_LF n M -> lc_t_n_LF (S n) M.
-intros; generalize dependent n;
-induction M; intros; inversion H; subst;
-eauto using lc_t_n_LF.
-Qed.
-
-Lemma closed_t_addition:
-forall M n m,
-  lc_t_n_LF n M -> lc_t_n_LF (n + m) M.
-intros; induction m;
-[ replace (n+0) with n by auto |
-  replace (n + S m) with (S (n+m)) by auto] ;
-try apply closed_t_succ;
-assumption.
-Qed.
-
-Lemma SL_nil:
-forall M,
-  SL nil M = M.
-induction M; intros; simpl in *;
-try erewrite IHM || (erewrite IHM1; erewrite IHM2); eauto.
-destruct v; auto.
-Qed.
-
-Lemma Mem_find_var:
-  forall L v,
-    Mem v (map fst_ (map fst_ L)) ->
-    exists A M, find_var L v = Some (v, A, M).
-induction L; intros; [ rewrite Mem_nil_eq in *; contradiction | ];
-destruct a; destruct p; rew_map in *; simpl in *.
-subst; rewrite Mem_cons_eq in H.
-destruct (eq_var_dec v v0).
-subst; simpl; exists t0 t; auto.
-destruct H; try contradiction; apply IHL; auto.
-Qed.
-
-Lemma NotMem_find_var:
-  forall L v,
-    ~Mem v (map fst_ (map fst_ L)) ->
-    find_var L v = None.
-induction L; intros; simpl in *; auto;
-destruct a; destruct p; rew_map in *; simpl in *;
-case_if.
-elim H; apply Mem_here.
-apply IHL; intro; elim H;
-rewrite Mem_cons_eq; right; auto.
-Qed.
-
-Lemma find_var_Mem:
-forall L v A M,
-  find_var L v = Some (v, A, M) -> Mem (v, A, M) L.
-induction L; intros; [inversion H; subst | ].
-destruct a; destruct p; simpl in *; case_if.
-inversion H; subst; apply Mem_here.
-rewrite Mem_cons_eq; right; apply IHL; auto.
-Qed.
-
-Lemma lc_SL:
-forall M L n,
-  lc_t_n_LF n M ->
-  (forall a b c, Mem (a,b,c) L -> lc_t_LF c) ->
-  lc_t_n_LF n (SL L M).
-induction M; intros; simpl in *;
-try (inversion H; subst; constructor; eapply IHM; eauto).
-destruct v; inversion H; subst.
-constructor; auto.
-destruct (Mem_dec var (map fst_ (map fst_ L)) v). apply eq_var_dec.
-apply Mem_find_var in m; destruct m; destruct H1.
-rewrite H1. replace n with (0+n) by omega.
-apply closed_t_addition; apply H0 with v x. apply find_var_Mem; auto.
-rewrite NotMem_find_var; auto.
-inversion H; subst; constructor; [apply IHM1 | apply IHM2]; auto.
-inversion H; subst; constructor; [eapply IHM2 | apply IHM1]; auto.
-Qed.
-
-Lemma SL_bte_subst:
-forall L0 M x k,
-  ~ Mem x (map fst_ (map fst_ L0)) ->
-  (forall v a m, Mem (v, a, m) L0 -> lc_t_LF m) ->
-  [hyp_LF (fte x) // bte k](SL L0 M) =
-  SL L0 [hyp_LF (fte x) // bte k]M.
-induction M; intros; simpl in *;
-try rewrite IHM || (rewrite IHM1; try rewrite IHM2); auto.
-case_if; simpl.
-case_if. rewrite NotMem_find_var; auto.
-destruct v; simpl; repeat case_if; auto.
-destruct (Mem_dec var (map fst_ (map fst_ L0)) v);
-try apply eq_var_dec; [ | rewrite NotMem_find_var]; auto;
-simpl; repeat case_if; auto.
-apply Mem_find_var in m; destruct m as (a, (b, m)); rewrite m; simpl.
-rewrite closed_subst_t_bound_LF with (n:=0); auto; try omega;
-apply H0 with v a; apply find_var_Mem; auto.
-Qed.
-
-Fixpoint FV_L (L: list (var * ty * te_LF)) :=
-match L with
-| nil => \{}
-| (v, A, M) :: L' => used_vars_te_LF M \u FV_L L'
-end.
-
-Lemma notin_FV_notin_elem:
-forall x L,
-  x \notin FV_L L ->
-  forall a b c, Mem (a,b,c) L -> x \notin used_vars_te_LF c.
-induction L; intros; simpl in *.
-rewrite Mem_nil_eq in *; contradiction.
-rewrite Mem_cons_eq in H0; destruct H0; [inversion H0; subst | ].
-rewrite notin_union in H; destruct H; auto.
-destruct a; destruct p; rewrite notin_union in H; destruct H;
-apply IHL with (a:=a0) (b:=b); auto.
-Qed.
-
-Lemma SL_extend:
-forall M L0 x A N,
-  x \notin FV_L L0 ->
-  ~Mem x (map fst_ (map fst_ L0)) ->
-  SL ((x, A, N) :: L0) M =
-  [N // fte x](SL L0 M).
-induction M; intros; simpl in *;
-try rewrite IHM || (rewrite IHM1; try rewrite IHM2); auto.
-destruct v; simpl; repeat case_if; auto.
-rewrite NotMem_find_var; auto; simpl; case_if; auto.
-destruct (Mem_dec var (map fst_ (map fst_ L0)) v);
-try apply eq_var_dec; [ | rewrite NotMem_find_var]; auto;
-simpl; repeat case_if; auto.
-apply Mem_find_var in m; destruct m as (a, (b, m)); rewrite m; simpl.
-rewrite closed_subst_t_free_LF; auto.
-apply notin_FV_notin_elem with L0 v a; eauto.
-apply find_var_Mem; eauto.
-Qed.
-
-Lemma Red_appl:
-forall M N A B,
-lc_t_LF (appl_LF M N) -> Red M (A ---> B) -> Red N A -> Red (appl_LF M N) B.
-intros; simpl in *; apply H0; inversion H; auto.
-Qed.
-
-Lemma Red_unbo:
-forall M A,
-Red M ([*]A) -> Red (unbox_LF M) A.
-intros; simpl in *; auto.
-Qed.
-
-Lemma Red_here:
-forall N A,
-lc_t_LF N -> Red N A -> Red (here_LF N) (<*>A).
-intros; simpl in *; intros; apply H3; auto.
-Qed.
-
-Lemma WT_letdia:
-forall K M N,
-  WT M ->
-  WT (ContAppl K ([M // bte 0]N)) ->
-  WT (ContAppl K (here_LF (letdia_LF (here_LF M) N))).
-Admitted.
-
-Theorem main_theorem:
-forall G Gamma M A,
-  lc_t_LF M ->
-  G |= Gamma |- M ::: A ->
- forall L,
-    concat(Gamma::G) *=* map fst_ L ->
-    (forall a b c, Mem (a,b,c) L -> lc_t_LF c) ->
-    (forall a b c, Mem (a,b,c) L -> Red c b) ->
-  forall K B,
-    ContTyping K A B ->
-    RedCont K A B ->
-    WT (ContAppl K (here_LF (SL L M))).
-intros G Gamma M A LC HT; induction HT; unfold RedCont in *;
-intros.
-(* hyp *)
-assert (lc_t_LF (SL L (hyp_LF (fte v)))) by
-  (apply lc_SL; auto; constructor);
-simpl in *;
-remember (match find_var L v with
-           | Some (_, _, M) => M
-           | None => hyp_LF (fte v)
-           end) as M';
-assert (Red M' A) by
-(subst; apply SL_hyp with G Gamma; auto; constructor; auto);
-apply H4 with (V:=M') in H3; auto.
-Focus 8.
-simpl.
-replace (ContAppl K (here_LF (letdia_LF (SL L0 M) (SL L0 N)))) with
- (ContAppl (ConsK K (SL L0 N) A B) (SL L0 M)) by (simpl; auto).
-remember (ConsK K (SL L0 N) A B) as K'.
-
-(* lam *)
+assert (WT (ContAppl (IdK (<*>A)) (here_LF (SL L0 M)))).
+  apply IHHT; auto. constructor.
+  unfold RedCont in *; intros; simpl. apply property_1 in H6; auto;
+  rewrite <- WT_here; auto.
+simpl in H6.
+assert (WT (SL L0 M)). rewrite WT_here; auto; apply lc_SL; auto.
+assert (exists V, SL L0 M |->* V /\ value_LF V).
+  inversion H7. subst; eexists; split; eauto; constructor.
+  destruct H8 as (V, (H8, H12)); subst. exists V; split; auto. skip.
+destruct H8 as (V, (H8, H12)).
+assert (exists V', V = here_LF (SL L0 V')). skip.
+destruct H10 as (V', H10); subst.
+apply WT_steps_back with
+(N:=ContAppl (ConsK K (SL L0 N) A B) (here_LF (SL L0 V'))).
+apply steps_KApplSteps; auto. constructor; auto; apply lc_SL; auto.
+apply lc_SL; auto. skip. (* from H8, need to make up my mind *)
+simpl. apply WT_step_back with
+  (N:=(ContAppl K (here_LF ((SL L0 N) ^t^ (SL L0 V'))))).
+Focus 2.
+unfold open_LF.
+apply Step_KApplStep; auto. repeat constructor; auto; apply lc_SL; auto.
+apply lc_t_steps_LF with M; auto. skip.
+constructor. skip. constructor. skip. skip.
+inversion H12; auto.
 unfold open_LF in *.
-assert (exists x, x \notin L \u used_vars_te_LF (SL L0 M) \u
-       from_list (map fst_ (map fst_ L0)) \u FV_L L0) by apply Fresh;
-destruct H6.
-assert (WT (ContAppl K (here_LF (SL L0 [hyp_LF (fte x) // bte 0]M)))).
-apply H0 with B0; eauto.
-apply lc_t_subst_t_LF_bound; [constructor | inversion LC]; auto.
-rewrite <- H1.
-
-specialize H0 with x L K B0.
-apply H5; auto; [ | apply lc_SL; auto].
-simpl in *; intros; unfold open_LF in *;
-assert (exists x, x \notin L \u used_vars_te_LF (SL L0 M) \u
-       from_list (map fst_ (map fst_ L0)) \u FV_L L0) by apply Fresh;
-destruct H6; simpl in *; intros; apply property_3.
-constructor; auto; constructor; apply lc_SL; auto; inversion LC; auto.
-constructor.
-intros; inversion H7; subst; [ | inversion H13];
+assert (exists v, v \notin L \u  used_vars_te_LF (SL L0 N) \u
+       from_list (map fst_ (map fst_ L0))\u FV_L L0)
+  by apply Fresh. destruct H10.
 rewrite subst_t_neutral_free_LF with (v:=x); auto.
-replace ([N // fte x]([hyp_LF (fte x) // bte 0](SL L0 M))) with
-  (SL ((x, A, N)::L0) [hyp_LF (fte x) // bte 0]M).
-
-(*apply H5; auto.
-rewrite SL_bte_subst; auto; [ | apply notin_Mem; auto].
-rewrite SL_extend; auto; apply notin_Mem; auto.
-(* appl *)
-simpl in *; inversion LC; subst; apply IHHT1; auto; apply lc_SL; auto.
-(* box *)
-simpl in *; inversion LC; subst; apply property_3.
-constructor; constructor; apply lc_SL; auto.
-constructor.
-intros; inversion H2; subst.
-apply IHHT; auto; rew_concat in *; rewrite <- H; permut_simpl.
-inversion H6.
-(* unbox *)
-simpl in *;
-inversion LC; subst; apply IHHT; auto.
-(* unbox-fetch *)
-simpl in *;
-inversion LC; subst; apply IHHT; auto;
-rewrite <- H0; apply PPermut_concat_permut; rewrite <- H; PPermut_LF_simpl.
-(* here *)
-inversion LC; subst; simpl in *; intros.
-apply H5; [ | apply lc_SL]; auto.
-(* get-here *)
-inversion LC; subst; simpl in *; intros.
-apply H6; [ | apply lc_SL]; auto.
-apply IHHT; auto.
-rewrite <- H0.
-apply PPermut_concat_permut; rewrite <- H; PPermut_LF_simpl.
-(* letdia *)
-unfold open_LF in *; simpl; inversion LC; subst.
-apply reducible_letdia with A.
-apply IHHT; auto.
-intros.
-assert (exists x, x\notin L) by apply Fresh.
-destruct H4.
-rewrite subst_t_neutral_free_LF with (v:=x); auto.
-replace ([P // fte x]([hyp_LF (fte x) // bte 0](SL L0 N))) with
-  (SL ((x, A, P)::L0) [hyp_LF (fte x) // bte 0]N).
-apply H with (G':=((x,A)::nil)::G); auto.
-skip. rew_map; rewrite <- H0; rew_concat; simpl; permut_simpl.
-skip. skip.
-rewrite SL_bte_subst; auto; [ | apply notin_Mem; auto].
-rewrite SL_extend; auto.
-skip. skip. skip. skip.
-rewrite
-
-Admitted.
-
-Lemma less_trivial_2:
-forall G Gamma M A,
-  lc_t_LF M ->
-  G |= Gamma |- M ::: A ->
-  Red M A ->
-  forall K B,
-    ContTyping K A B ->
-    WT (ContAppl K (here_LF M)).
-Admitted.
-
-Lemma non_trivial:
-forall G Gamma M A,
-  lc_t_LF M ->
-  G |= Gamma |- M ::: A ->
-  forall K B,
-    ContTyping K A B ->
-    WT (ContAppl K (here_LF M)).
-Admitted.
-*)
-
-(* Theorem:
-forall G Gamma M A,
-  lc_t_LF M ->
-  G |= Gamma |- M ::: A ->
-  forall K B, ContTyping K A B -> WT (ContAppl K (here_LF M)).
-intros G Gamma M A LC HT; induction HT; intros.
-*)
-
+rewrite SL_bte_subst; [ | apply notin_Mem |]; eauto.
+rewrite <- SL_extend with (A:=A); auto.
+Focus 2. apply notin_Mem; auto.
+apply H with (G':= ((x, A) :: nil) :: G); auto.
+apply lc_t_subst_t_LF_bound; auto; constructor.
+constructor. rewrite Mem_nil_eq; auto. apply OkL_fresh; auto.
+rewrite from_list_nil. rewrite union_empty_r. auto.
+rew_map in *; simpl; rewrite <-  H1; rew_concat; auto. permut_simpl.
+intros; rewrite Mem_cons_eq in *; destruct H13; eauto;
+inversion H13; subst; auto. apply lc_SL; auto. skip.
+intros; rewrite Mem_cons_eq in *; destruct H13; eauto;
+inversion H13; subst; auto.
+(* Red (SL L0 V') A - srsly?! *)
+skip. (* :( *)
+(* letdia-get*)
+skip. (* same old.. *)
+Qed.
 Lemma lc_t_n_LF_subst_t:
 forall N M n,
 lc_t_n_LF n M ->
@@ -1775,6 +967,11 @@ specialize H0 with x; apply H0 in H2;
 apply lc_t_n_LF_subst_t in H2; auto; constructor.
 Qed.
 
+Lemma SL_nil:
+forall M,
+  SL nil M = M.
+Admitted.
+
 Theorem WT_Lang:
 forall G M A,
   emptyEquiv_LF G |= nil |- M ::: A ->
@@ -1783,16 +980,15 @@ intros.
 assert (lc_t_LF M).
   apply types_LF_lc_t_LF in H; auto.
 assert (WT (ContAppl (IdK A) (here_LF M))).
-apply less_trivial_1 with (L:=nil) (K:=IdK A) (B:=A) in H; auto.
+apply main_theorem with (L:=nil) (K:=IdK A) in H; auto.
 rewrite SL_nil in H; auto.
+constructor.
 rew_concat; rew_map; clear M A H H0;
 induction G; simpl; rew_concat; auto.
 intros; rewrite Mem_nil_eq in *; contradiction.
 intros; rewrite Mem_nil_eq in *; contradiction.
 constructor.
 unfold RedCont; intros; simpl.
-repeat apply WT_N_WT_here; apply property_1 with (A:=A); auto.
-simpl in H1; apply WT_here; [constructor |]; auto; apply WT_here; auto;
-constructor; constructor; auto.
+apply property_1 in H1; auto. rewrite <- WT_here; auto.
+simpl in H1; apply WT_here; auto.
 Qed.
-*)
